src/parser/parseit.fs
@@ -51,31 +51,33 @@ let read_build_config (filename:string) =
         let fields = bc.Split([|';'|]) in
         fields |> Array.iter (fun field -> 
         let field = field.Trim() in
-        let nv = field.Split([|':'|]) in
-        if nv.Length <> 2 
-        then fail ("could not parse field: " ^ field)
-        else let name, value = nv.(0), nv.(1) in
-             match name with 
-                | "options" -> set_options value
-                | "other-files" -> 
-                    set_filenames (Util.split value " " 
-                                    |> List.collect 
-                                        (fun x ->
-                                        let x = Util.trim_string x in
-                                        if String.length x = 0
-                                        then []
-                                        else [x]))
-                | "variables" -> 
-                  let vars = value.Split([|' '|]) in 
-                  vars |> Array.iter (fun v -> 
-                    let v = Util.trim_string v in
-                    if String.length v = 0
-                    then ()
-                    else let xv = v.Split([|'='|]) in
-                         if xv.Length <> 2
-                         then fail ("could not parse variable: " ^ v)
-                         else set_variable (xv.(0).Trim(), xv.(1).Trim()))
-                | _ -> fail ("unexpected config option: " ^ name));
+        if field = "" then ()
+        else
+            let nv = field.Split([|':'|]) in
+            if nv.Length <> 2 
+            then fail ("could not parse field: " ^ field)
+            else let name, value = nv.(0), nv.(1) in
+                 match name with 
+                    | "options" -> set_options value
+                    | "other-files" -> 
+                        set_filenames (Util.split value " " 
+                                        |> List.collect 
+                                            (fun x ->
+                                            let x = Util.trim_string x in
+                                            if String.length x = 0
+                                            then []
+                                            else [x]))
+                    | "variables" -> 
+                      let vars = value.Split([|' '|]) in 
+                      vars |> Array.iter (fun v -> 
+                        let v = Util.trim_string v in
+                        if String.length v = 0
+                        then ()
+                        else let xv = v.Split([|'='|]) in
+                             if xv.Length <> 2
+                             then fail ("could not parse variable: " ^ v)
+                             else set_variable (xv.(0).Trim(), xv.(1).Trim()))
+                    | _ -> fail ("unexpected config option: " ^ name));
 
         begin match !options with 
             | None -> ()
